theories/rust_typing/integration_tests.v
@@ -182,6 +182,9 @@ Section test.
   Next Obligation. ex_t_solve_timeless. Qed.
   Local Definition Pty := (∃; Pdef, int I32)%I.
 
+  Local Lemma Pty_copy : Copyable Pty.
+  Proof. apply _. Qed.
+
   Local Definition P_b := λ (π : thread_id) (x : Z) (y : Z), (∃ (z : Z) (l : loc), ⌜x = (y + z)%Z⌝ ∗ ⌜(0 < x)%Z⌝ ∗ guarded true (l ◁ₗ[π, Owned] #42%Z @ (◁ int I32)))%I : iProp Σ.
   Local Definition S_b := λ (π : thread_id) (κ : lft) (x : Z) (y : Z), (∃ (z : Z) (l : loc), ⌜x = (y + z)%Z⌝ ∗ ⌜(0 < x)%Z⌝ ∗ guarded false (l ◁ₗ[π, Shared κ] #42%Z @ (◁ int I32)))%I : iProp Σ.
 
